theories/theories/utp_reactive.thy
@@ -79,11 +79,13 @@ proof -
   also have "... = `(II\<^bsub>rea\<^esub> \<and> ($tr \<le> $tr\<acute>)) \<lhd> $wait \<rhd> (P \<and> ($tr \<le> $tr\<acute>))`" by (utp_pred_auto_tac)
   ultimately show ?thesis by (simp add:SkipREA_is_R1, utp_rel_tac)
 qed
-  
+
 lemma R1_R2_commute : "R1 (R2 P) = R2 (R1 P)" 
 proof -
   have "R2 (R1 P) = `(P \<and> ($tr \<le> $tr\<acute>))[\<langle>\<rangle>/tr][($tr\<acute> - $tr)/tr\<acute>]`" by (utp_rel_tac)
-  also have "... = `P[\<langle>\<rangle>/tr][($tr\<acute> - $tr)/tr\<acute>] \<and> ($tr \<le> $tr\<acute>)`" sorry(*by (simp add:usubst erasure typing defined closure R1_true_is_R2)*)
+  also have "... = `P[\<langle>\<rangle>/tr][($tr\<acute> - $tr)/tr\<acute>] \<and> ($tr \<le> $tr\<acute>)`" 
+    apply (simp add:usubst closure typing defined)
+sorry(*by (simp add:usubst erasure typing defined closure R1_true_is_R2)*)
   ultimately show ?thesis by (utp_rel_tac)
 qed
 lemma R2_R3_commute : "R2 (R3 P) = R3 (R2 P)" 
